DP_Pred.thy
@@ -1,0 +1,14 @@
+theory DP_Pred
+  imports "./DP_Consistency"
+begin
+context dp_consistency
+begin
+context 
+  includes lifting_syntax
+begin
+  
+  
+  
+end
+end
+end
