scratch/Scratch.thy
@@ -1,5 +1,10 @@
 theory Scratch
   imports Main
 begin
-  term int
+term int
+term fold
+  
+fun f :: "nat \<Rightarrow> nat" where
+  "f 0 = 0"
+| "f (Suc x) = fold op + (map (\<lambda>x. f) [0..<x]) 0"
 end
